Rename

specIR/SIRHoareproof.v
@@ -18,7 +18,7 @@ Require Import Mod ModSem Any Skeleton.
 Require Import SimMem SimSymb Sound.
 Require SimMemId SimSymbId SoundTop.
 Require Import SimMod SimModSem.
-Require Import SIRCommon SIR.
+Require Import SIRCommon SimSIR SIR.
 
 Require Import Program.
 Require Import Simulation.
@@ -44,6 +44,7 @@ Variable mi: string.
 Variable owned_heap: Type.
 Variable precond: owned_heap -> mem -> list val -> Prop.
 Variable postcond: owned_heap -> mem -> list val -> (owned_heap * (mem * val)) -> Prop.
+Let sim_st := sim_st (@eq owned_heap).
 
 
 
@@ -64,27 +65,39 @@ Section SYNTAX.
 
 (*** sim itree ***)
 Let itr := itree (E owned_heap) (owned_heap * (mem * val)).
+Variable _fn _fn_ru: ident.
 
-Inductive _sim_itr (sim_itr: itr -> itr -> Prop): itr -> itr -> Prop :=
-| sim_ret
+(*** TODO: We don't have to define these in coinductive manner. Try inductive style instead? SimSIRLocal also. ***)
+(*** TODO: However, if we want to add loop, we may need coinductive...? Q: Why loop and recursion is treated differently? ***)
+Inductive _match_itr (match_itr: itr -> itr -> Prop): itr -> itr -> Prop :=
+| match_ret
     oh m v
   :
-    _sim_itr sim_itr (Ret (oh, (m, v))) (Ret (oh, (m, v)))
-| sim_tau
+    _match_itr match_itr (Ret (oh, (m, v))) (Ret (oh, (m, v)))
+| match_tau
     i_src
     i_tgt
-    (SIM: sim_itr i_src i_tgt)
+    (MATCH: match_itr i_src i_tgt)
   :
-    _sim_itr sim_itr (Tau i_src) (Tau i_tgt)
-| sim_icall
+    _match_itr match_itr (Tau i_src) (Tau i_tgt)
+| match_icall
     fname oh0 m0 vs0 k_src k_tgt
-    (SIM: (eq ==> sim_itr)%signature k_src k_tgt)
+    (NEQ: fname <> _fn)
+    (NEQ: fname <> _fn_ru)
+    (MATCH: (eq ==> match_itr)%signature k_src k_tgt)
   :
-    _sim_itr sim_itr
+    _match_itr match_itr
+             (Vis (subevent _ (ICall fname oh0 m0 vs0)) k_src)
+             (Vis (subevent _ (ICall fname oh0 m0 vs0)) k_tgt)
+| match_icall_fn
+    oh0 m0 vs0 k_src k_tgt
+    (MATCH: (eq ==> match_itr)%signature k_src k_tgt)
+  :
+    _match_itr match_itr
              (* (Vis (subevent _ (ICall fname oh0 m0 vs0)) k_src) *)
-             (trigger (ICall fname oh0 m0 vs0) >>= k_src)
+             (trigger (ICall _fn_ru oh0 m0 vs0) >>= k_src)
              (guarantee (precond oh0 m0 vs0) ;;
-              ohmv <- trigger (ICall fname oh0 m0 vs0) ;;
+              ohmv <- trigger (ICall _fn oh0 m0 vs0) ;;
               assume (postcond oh0 m0 vs0 ohmv) ;;
               k_tgt ohmv
               (*** we can write in point-free style but ***)
@@ -95,56 +108,55 @@ Inductive _sim_itr (sim_itr: itr -> itr -> Prop): itr -> itr -> Prop :=
       (* guarantee (precond oh0 m0 vs0) ;; *)
       (* '(oh1, (m1, y1)) <- trigger (ICall _fib oh0 m0 vs0) ;; *)
       (* (assume (postcond oh0 m0 vs0 (oh1, (m1, y1)))) ;; *)
-| sim_ecall
+| match_ecall
     sg oh m vs fptr
     k_src
     k_tgt
-    (SIM: (eq ==> sim_itr)%signature k_src k_tgt)
+    (MATCH: (eq ==> match_itr)%signature k_src k_tgt)
   :
-    _sim_itr sim_itr
+    _match_itr match_itr
              (Vis (subevent _ (ECall sg fptr oh m vs)) k_src)
              (Vis (subevent _ (ECall sg fptr oh m vs)) k_tgt)
-| sim_nb
+| match_nb
     i_src k_tgt
   :
-    _sim_itr sim_itr i_src (Vis (subevent _ (ENB)) k_tgt)
-| sim_ub
+    _match_itr match_itr i_src (Vis (subevent _ (ENB)) k_tgt)
+| match_ub
     k_src i_tgt
   :
-    _sim_itr sim_itr (Vis (subevent _ (EUB)) k_src) i_tgt
-| sim_choose
+    _match_itr match_itr (Vis (subevent _ (EUB)) k_src) i_tgt
+| match_choose
     X
     k_src k_tgt
-    (SIM: (eq ==> sim_itr)%signature k_src k_tgt)
+    (MATCH: (eq ==> match_itr)%signature k_src k_tgt)
   :
-    _sim_itr sim_itr
+    _match_itr match_itr
              (Vis (subevent _ (EChoose X)) k_src)
              (Vis (subevent _ (EChoose X)) k_tgt)
 .
 
-Definition sim_itr: itr -> itr -> Prop := paco2 _sim_itr bot2.
+Definition match_itr: itr -> itr -> Prop := paco2 _match_itr bot2.
 
-Lemma sim_itr_mon: monotone2 _sim_itr.
+Lemma match_itr_mon: monotone2 _match_itr.
 Proof.
   ii. inv IN; try econs; et; rr; et.
 Unshelve.
 Qed.
-Hint Unfold sim_itr.
-Hint Resolve sim_itr_mon: paco.
+Hint Unfold match_itr.
+Hint Resolve match_itr_mon: paco.
 
 Section PROG.
 
-Variable _fn_ru: ident.
 Definition fn_src (oh0: owned_heap) (m0: mem) (vs0: list val): itree (E owned_heap) (owned_heap * (mem * val)) :=
   assume (precond oh0 m0 vs0) ;;
   _I_DONT_USE_THIS__RUDIMENT_ORGAN_ <- trigger (ICall _fn_ru oh0 m0 vs0) ;;
   trigger (EChoose { ohmv: (owned_heap * (mem * val)) | postcond oh0 m0 vs0 ohmv }) >>= (fun x => Ret (proj1_sig x))
 .
 
-Inductive sim_fn (fn_ru fn_tgt: function owned_heap): Prop :=
-| sim_fn_intro
+Inductive match_fn (fn_ru fn_tgt: function owned_heap): Prop :=
+| match_fn_intro
     fn_tgt_inner
-    (SIM: (eq ==> eq ==> eq ==> sim_itr) fn_ru fn_tgt_inner)
+    (SIM: (eq ==> eq ==> eq ==> match_itr) fn_ru fn_tgt_inner)
     (TGT: fn_tgt = fun oh0 m0 vs0 =>
                      assume (precond oh0 m0 vs0) ;;
                      (fn_tgt_inner oh0 m0 vs0)
@@ -152,18 +164,17 @@ Inductive sim_fn (fn_ru fn_tgt: function owned_heap): Prop :=
     )
 .
 
-Inductive sim_prog (p_src p_tgt: program owned_heap): Prop :=
-| sim_prog_intro
-    _fn
+Inductive match_prog (p_src p_tgt: program owned_heap): Prop :=
+| match_prog_intro
     fn_ru (* rudiment *) fn_tgt
     (FNSRC: p_src _fn = Some fn_src)
     (FNTGT: p_tgt _fn = Some fn_tgt)
     (RDSRC: p_src _fn_ru = Some fn_ru)
     (RDTGT: p_tgt _fn_ru = None)
-    (SIMFN: sim_fn fn_ru fn_tgt)
+    (SIMFN: match_fn fn_ru fn_tgt)
     (OTHERS: forall _fm (NEQ: _fm <> _fn) (NEQ: _fm <> _fn_ru), p_src _fm = p_tgt _fm)
   :
-    sim_prog p_src p_tgt
+    match_prog p_src p_tgt
 .
 
 End PROG.
@@ -177,7 +188,7 @@ End PROG.
 Inductive bindC (r: itr -> itr -> Prop) : itr -> itr -> Prop :=
 | bindC_intro
     i_src i_tgt
-    (SIM: sim_itr i_src i_tgt)
+    (SIM: match_itr i_src i_tgt)
     k_src k_tgt
     (SIMK: (eq ==> r) k_src k_tgt)
     (* (SIMK: forall *)
@@ -194,7 +205,7 @@ Hint Constructors bindC: core.
 Lemma bindC_spec
       simC
   :
-    bindC <3= gupaco2 (_sim_itr) (simC)
+    bindC <3= gupaco2 (_match_itr) (simC)
 .
 Proof.
   gcofix CIH. intros. destruct PR.
@@ -203,27 +214,35 @@ Proof.
   - rewrite ! bind_tau. gstep. econs; eauto. pclearbot.
     (* gfinal. left. eapply CIH. econstructor; eauto. *)
     debug eauto with paco.
-  - rewrite ! bind_bind. gstep.
-    erewrite f_equal3; try eapply sim_icall; revgoals.
-    { f. f_equiv. ii. f_equiv. ii. f. des_u.
-      rewrite bind_bind. refl. }
-    { refl. }
-    { refl. }
-    ii. clarify.
-    exploit (SIM0 y); eauto. intro R. pclearbot.
-    (* gbase. apply CIH. econs; eauto. *)
+  - irw. gstep; econs; et. ii. clarify. exploit (MATCH y); eauto. intro R. pclearbot.
     eauto with paco.
-  - rewrite ! bind_vis. gstep. econs; eauto. u. ii. clarify. exploit (SIM0 y); eauto. intro T. pclearbot.
+  - rewrite ! bind_bind. gstep. erewrite f_equal2; [eapply match_icall_fn|..]; try refl; cycle 1.
+    { f. f_equiv. ii. f_equiv. ii. f. instantiate (1:= k_src0 >>> k_src). irw.
+      f. f_equiv. ii. f_equiv; eauto. ii.
+    match_icall_fn
+    econs; eauto. u. ii. clarify. exploit (MATCH y); eauto. intro T. pclearbot.
     (* gfinal. left. eapply CIH. econs. { et. } uh. ii. eapply SIMK. et. *)
     eauto with paco.
+
+    
+             (trigger (ICall _fn_ru oh0 m0 vs0) >>= k_src)
+             (guarantee (precond oh0 m0 vs0) ;;
+              ohmv <- trigger (ICall _fn oh0 m0 vs0) ;;
+              assume (postcond oh0 m0 vs0 ohmv) ;;
+              k_tgt ohmv
+              (*** we can write in point-free style but ***)
+              (* trigger (ICall fname oh0 m0 vs0) *)
+              (* >>= assumeK (postcond oh0 m0 vs0) *)
+              (* >>= k_tgt *)
+             )
   - rewrite ! bind_vis. gstep. econs; eauto.
   - rewrite ! bind_vis. gstep. econs; eauto.
   - rewrite ! bind_vis. gstep. econs; eauto.
-    ii. clarify. exploit (SIM0 y); eauto. intro R. pclearbot. eauto with paco.
+    ii. clarify. exploit (MATCH y); eauto. intro R. pclearbot. eauto with paco.
 Qed.
 
-Global Instance sim_itr_bind :
-  Proper ((eq ==> sim_itr) ==> sim_itr ==> sim_itr) ITree.bind'
+Global Instance match_itr_bind :
+  Proper ((eq ==> match_itr) ==> match_itr ==> match_itr) ITree.bind'
 .
 Proof.
   red. ginit.
@@ -235,86 +254,8 @@ Proof.
 Qed.
 
 End SYNTAX.
-Hint Unfold sim_itr.
-Hint Resolve sim_itr_mon: paco.
-
-
-
-
-
-
-
-
-
-(*** sim semantics ***)
-Section SEMANTICS.
-
-(*** sim states ***)
-Let st := (SIR.state owned_heap).
-
-Inductive _sim_st (sim_st: st_src -> st_tgt -> Prop): st_src -> st_tgt -> Prop :=
-| sim_st_ret
-    oh_src oh_tgt m v
-    (O: SO oh_src oh_tgt)
-  :
-    _sim_st sim_st (Ret (oh_src, (m, v))) (Ret (oh_tgt, (m, v)))
-| sim_st_tau
-    i_src
-    i_tgt
-    (SIM: sim_st i_src i_tgt)
-  :
-    _sim_st sim_st (Tau i_src) (Tau i_tgt)
-| sim_st_ecall
-    sg m vs fptr
-    oh_src k_src
-    oh_tgt k_tgt
-    (O: SO oh_src oh_tgt)
-    (SIM: HProper (SALL !-> sim_st) k_src k_tgt)
-  :
-    _sim_st sim_st
-             (Vis (subevent _ (ECall sg fptr oh_src m vs)) k_src)
-             (Vis (subevent _ (ECall sg fptr oh_tgt m vs)) k_tgt)
-| sim_st_nb
-    i_src k_tgt
-  :
-    _sim_st sim_st i_src (Vis (subevent _ (ENB)) k_tgt)
-| sim_st_ub
-    k_src i_tgt
-  :
-    _sim_st sim_st (Vis (subevent _ (EUB)) k_src) i_tgt
-| sim_st_choose_src
-    X_src
-    k_src i_tgt
-    (SIM: exists x_src, sim_st (k_src x_src) i_tgt)
-  :
-    _sim_st sim_st
-            (Vis (subevent _ (EChoose X_src)) k_src)
-            (Tau i_tgt)
-| sim_st_choose_tgt
-    X_tgt
-    k_tgt i_src
-    (INHAB: inhabited X_tgt)
-    (SIM: forall x_tgt, sim_st i_src (k_tgt x_tgt))
-  :
-    _sim_st sim_st
-            (Tau i_src)
-            (Vis (subevent _ (EChoose X_tgt)) k_tgt)
-.
-
-Definition sim_st: st_src -> st_tgt -> Prop := paco2 _sim_st bot2.
-
-Lemma sim_st_mon: monotone2 _sim_st.
-Proof.
-  ii. inv IN; try econs; et.
-  des. esplits; et.
-Unshelve.
-Qed.
-Hint Unfold sim_st.
-Hint Resolve sim_st_mon: paco.
-
-End SEMANTICS.
-Hint Unfold sim_st.
-Hint Resolve sim_st_mon: paco.
+Hint Unfold match_itr.
+Hint Resolve match_itr_mon: paco.
 
 
 
@@ -325,13 +266,13 @@ Hint Resolve sim_st_mon: paco.
 
 Section SIM.
 
-  Variable p_src: program owned_heap_src.
-  Variable p_tgt: program owned_heap_tgt.
-  Hypothesis (SIMP: sim_prog p_src p_tgt).
+  Variable p_src: program owned_heap.
+  Variable p_tgt: program owned_heap.
+  Hypothesis (SIMP: match_prog p_src p_tgt).
 
   Lemma sim_prog_sim_st
         i_src i_tgt
-        (SIM: sim_itr i_src i_tgt)
+        (SIM: match_itr i_src i_tgt)
     :
       sim_st (interp_mrec (interp_function p_src) i_src)
              (interp_mrec (interp_function p_tgt) i_tgt)
@@ -346,13 +287,14 @@ Section SIM.
     - gstep. econs; et.
     - pclearbot. gstep. econs; et. gbase. et.
     - pclearbot. gstep. econs; et. gbase.
-      eapply CIH. eapply sim_itr_bind.
-      { u. ii. repeat spc SIM0. pclearbot. eauto. }
+      eapply CIH. eapply match_itr_bind.
+      { u. ii. repeat spc MATCH. pclearbot. eauto. }
       exploit (@SIMP fname); et. intro T.
       inv T.
       { pfold. econs; et. }
       exploit H1; et.
-    - gstep. econs; et. u in *. gstep. econs; et. repeat spc SIM0. des; ss. gbase. eapply CIH.
+    - gstep. econs; et. u in *. gstep. econs; et. repeat spc MATCH. specialize (MATCH H0).
+      des; ss. gbase. eapply CIH.
       eauto with paco.
     - gstep. econs; et.
     - gstep. econs; et.
@@ -368,8 +310,8 @@ Section SIM.
       (fname: ident) m vs oh_src oh_tgt
       (O: SO oh_src oh_tgt)
     ,
-      (<<SIM: sim_st (interp_program0 p_src (ICall fname oh_src m vs))
-                     (interp_program0 p_tgt (ICall fname oh_tgt m vs))
+      (<<SIM: sim_st (interp_program p_src (ICall fname oh_src m vs))
+                     (interp_program p_tgt (ICall fname oh_tgt m vs))
                      >>)
   .
   Proof.
@@ -382,54 +324,6 @@ Section SIM.
     }
   Qed.
 
-  (*** lifting above proof into small-step semantics ***)
-  Section SMO.
-
-    Record t: Type :=
-      mk {
-          sm :> SimMem.t;
-          oh_src: Any;
-          oh_tgt: Any;
-        }
-    .
-
-    Inductive wf (smo: t): Prop :=
-    | wf_intro
-        (o_src: owned_heap_src) (o_tgt: owned_heap_tgt)
-        (MWF: SimMem.wf smo)
-        (OHSRC: smo.(oh_src) = upcast o_src)
-        (OHTGT: smo.(oh_tgt) = upcast o_tgt)
-        (O: SO o_src o_tgt)
-    .
-
-    Local Obligation Tactic := try (by ii; des; ss).
-
-    Program Instance SimMemOh: (SimMemOh.class) :=
-      {|
-      SimMemOh.t := t;
-      SimMemOh.sm := sm;
-      SimMemOh.oh_src := oh_src;
-      SimMemOh.oh_tgt := oh_tgt;
-      SimMemOh.wf := wf;
-      SimMemOh.le := SimMem.le;
-      SimMemOh.lepriv := SimMem.lepriv;
-      SimMemOh.midx := Some mi;
-      SimMemOh.set_sm := fun smo sm => mk sm smo.(oh_src) smo.(oh_tgt);
-      |}
-    .
-    Next Obligation.
-      ii. eapply PR.
-    Qed.
-    Next Obligation.
-      ii. inv WF.
-      econs; ss; et.
-    Qed.
-    Next Obligation.
-      ss. ii. destruct smo0; ss.
-    Qed.
-
-  End SMO.
-
   Variable ioh_src: SkEnv.t -> owned_heap_src.
   Variable ioh_tgt: SkEnv.t -> owned_heap_tgt.
   Hypothesis (SIMO: forall skenv, SO (ioh_src skenv) (ioh_tgt skenv)).
@@ -437,170 +331,15 @@ Section SIM.
   Let md_src: Mod.t := (SIR.module sk p_src mi ioh_src).
   Let md_tgt: Mod.t := (SIR.module sk p_tgt mi ioh_tgt).
 
-
-
-  (*** Lifting to SimModSem ***)
-  Section SIMMODSEM.
-
-    Variable skenv_link: SkEnv.t.
-    Variable sm_link: SimMem.t.
-    Let ms_src: ModSem.t := (Mod.modsem md_src skenv_link).
-    Let ms_tgt: ModSem.t := (Mod.modsem md_tgt skenv_link).
-    Hypothesis (INCL: SkEnv.includes skenv_link (Mod.sk md_src)).
-    Hypothesis (WF: SkEnv.wf skenv_link).
-
-    Local Existing Instance SimMemOh.
-    Local Arguments ModSemPair.mk [SM] [SS] _ _ _ _ [SMO].
-
-    Definition msp: ModSemPair.t := ModSemPair.mk (md_src skenv_link) (md_tgt skenv_link)
-                                                  (SimSymbId.mk md_src md_tgt) sm_link.
-
-    Inductive match_states (idx: nat): SIR.state owned_heap_src ->
-                                       SIR.state owned_heap_tgt -> SimMemOh.t -> Prop :=
-    | match_states_intro
-        st_src st_tgt smo0
-        (SIM: sim_st st_src st_tgt)
-        (MWF: SimMemOh.wf smo0)
-      :
-        match_states idx st_src st_tgt smo0
-    .
-
-    Lemma match_states_lxsim
-          idx st_src_src st_tgt_src smo_src
-          (MATCH: match_states idx st_src_src st_tgt_src smo_src)
-      :
-        <<XSIM: lxsim (md_src skenv_link) (md_tgt skenv_link)
-                      (fun _ => () -> exists (_ : ()) (_ : mem), True)
-                      (Ord.lift_idx lt_wf idx) st_src_src st_tgt_src smo_src>>
-    .
-    Proof.
-      revert_until idx. revert idx.
-      ginit.
-      { intros. eapply cpn4_wcompat; eauto with paco. }
-      gcofix CIH. i. gstep.
-      ii. clear SUSTAR.
-
-      inv MATCH. ss.
-      punfold SIM. inv SIM.
-      - assert(U:=MWF).
-        inv MWF. inv MWF0. destruct smo_src; ss. destruct sm0; ss. clarify.
-        econstructor 4 with (smo_ret := mk (SimMemId.mk m m)
-                                           (upcast oh_src0) (upcast oh_tgt0)); ss; eauto.
-        + econs; ss; et.
-        + econs; ss; et.
-        + econs; ss; et.
-        + rr. ss. esplits; ss; et.
-          { econs; ss; et. }
-      - (* TAU *)
-        econs 1; et.
-        econs 1; et; swap 2 3.
-        { split; intro T; rr in T; des; ss; inv T; ss. }
-        { eapply modsem_receptive; et. }
-        ii; ss. inv STEPSRC; ss. clarify. esplits; ss; et.
-        { left. eapply plus_one. rr. esplits; et.
-          { eapply modsem_determinate; ss; et. }
-          econs; et.
-        }
-        pclearbot. gbase. eapply CIH. econs; et.
-      - (* ECALL *)
-        econs 3; et.
-        { admit "TODO: fix -- ~step, ~ret should suffice". }
-        ii; ss. inv ATSRC. csc.
-        eexists _, _, (mk (SimMemId.mk m0 m0) (upcast oh_src1) (upcast oh_tgt0)); ss.
-        esplits; ss; et.
-        { rr. ss. esplits; ss; et. econs; ss; et. }
-        { econs; ss; et. }
-        { econs; ss; et. }
-        ii. des. inv AFTERSRC; ss. inv GETK; ss. csc.
-        rename oh_src0 into oh_src1.
-        rename _oh0 into oh_src0.
-        rr in SIMRETV. des; ss. inv SIMRETV0; ss. clarify.
-        inv MWF0. ss. destruct smo_ret; ss. destruct sm0; ss. subst. clarify. clear_tac.
-        esplits; et.
-        { econs; ss; et. econs; ss; et. }
-        u in SIM0.
-        hexploit SIM0; et.
-        { instantiate (2:= (o_src, (_, _))). instantiate (1:= (o_tgt, (_, _))). ss. }
-        intro T. des; ss.
-        gbase. eapply CIH. econs; et.
-      - (* NB *)
-        econs 2; ss; et. ii.
-        econs 3; ss; et.
-        { ii; ss. inv STEPTGT; ss. }
-        { esplits; et. econsby ss. }
-      - (* UB *)
-        econs 2; ss; et. ii.
-        exploit SAFESRC; et.
-        { eapply star_refl. }
-        intro T; des; ss.
-        + rr in EVCALL. des; ss. inv EVCALL; ss.
-        + rr in EVRET. des; ss. inv EVRET; ss.
-        + inv EVSTEP; ss.
-      - (* CHOOSE SRC *)
-        des. pclearbot.
-        econs 2; ss; et. ii.
-        econs 1; ss; et; cycle 1.
-        { esplits; ss; et. econs; ss; et. }
-        { ii. inv STEPTGT; ss; clarify. esplits; et.
-          + left. eapply plus_one. econs 3; ss; et.
-          + gbase. eapply CIH. econs; et.
-        }
-      - (* CHOOSE TGT *)
-        des. pclearbot. inv INHAB.
-        econs 2; ss; et. ii.
-        econs 1; ss; et; cycle 1.
-        { esplits; ss; et. econs 3; ss; et. }
-        { ii. inv STEPTGT; ss; csc. esplits; et.
-          + left. eapply plus_one. econs; ss; et.
-          + gbase. eapply CIH. econs; et.
-        }
-    Unshelve.
-      all: ss.
-      all: try (econsby ss).
-    Qed.
-
-    Theorem sim_modsem: ModSemPair.sim msp.
-    Proof.
-      econstructor 1 with (sidx := unit) (sound_states := top4); eauto;
-        try apply SoundTop.sound_state_local_preservation; et; try (by ii; ss).
-      { ii. eapply Preservation.local_preservation_noguarantee_weak.
-        apply SoundTop.sound_state_local_preservation; et.
-      }
-      { ii. ss. eexists (mk _ _ _); ss. esplits; eauto. econs; ss; eauto. }
-      ii. ss. esplits; eauto.
-      - ii. des. inv INITTGT. inv SAFESRC. ss. des_ifs_safe.
-        esplits; eauto.
-        { econs; ss; et. }
-        eapply match_states_lxsim; eauto.
-        econs; ss; et.
-        eapply sim_prog_sim_st; et.
-        rr in SIMARGS. des. inv SIMARGS0; ss. clarify. inv MWF. ss. destruct sm_arg; ss.
-        destruct sm0; ss. subst. clarify. clear_tac.
-        assert(fid0 = fid).
-        { apply_all_once Genv.find_invert_symbol. clarify. }
-        clarify.
-        rr in SIMP. repeat spc SIMP. hexploit1 SIMP; et. inv SIMP; ss.
-        { pfold. econs; et. }
-        { eapply H1; et. }
-      - i; des. inv SAFESRC. ss. des_ifs.
-        rr in SIMARGS. des. inv SIMARGS0; ss. clarify. destruct sm_arg; ss. destruct sm0; ss. clarify.
-        esplits; et. econs; ss; et.
-    Unshelve.
-      all: ss.
-      all: try (econsby ss).
-    Qed.
-
-  End SIMMODSEM.
-
   Theorem sim_mod: ModPair.sim (SimSymbId.mk_mp (SIR.module sk p_src mi ioh_src)
                                                 (SIR.module sk p_tgt mi ioh_tgt)).
   Proof.
     ii. econs; ss; eauto.
     ii. rr in SIMSKENVLINK. clarify. esplits. eapply sim_modsem; et.
+    eapply adequacy_local_local.
   Qed.
 
 End SIM.
-
 End OWNEDHEAP.
 Hint Unfold sim_itr.
 Hint Resolve sim_itr_mon: paco.
